theories/Logic/Semantics.v
@@ -210,8 +210,6 @@ Module CtlNotations.
   Notation "'vis' R" := (CBase (vis_with R)) (in custom ctl at level 74): ctl_scope.
   Notation "'finish' R" := (CBase (finish_with R)) (in custom ctl at level 74): ctl_scope.
   Notation "'done' R" := (CBase (done_with R)) (in custom ctl at level 74): ctl_scope.
-  Notation "'doneS' R" := (CBase (done_with (fun '(r, s) w => R r w s)))
-                            (in custom ctl at level 74): ctl_scope.
   Notation "'done=' r w" := (CBase (done_with (fun r' w' => r = r' /\ w = w')))
                                 (in custom ctl at level 74): ctl_scope.
   
